Exercise 0.6-1: inductive, htmap2.
I don't understand the definition of htmap2 I've written by trial and
error.  I don't understand dependent pattern matching :(

0.6-1.v
@@ -23,7 +23,7 @@ Section htree.
   Variable elm : A.
 
   Inductive path : tree A -> Type :=
-  | Finish : path (Leaf elm)
+  | Stop : path (Leaf elm)
   | Left : forall l r, path l -> path (Node l r)
   | Right : forall l r, path r -> path (Node l r).
 
@@ -34,7 +34,7 @@ Section htree.
                                    | Leaf x => B x -> B elm
                                    | Node _ _ => unit
                                    end) with
-        | Finish => fun b => b
+        | Stop => fun b => b
         | Left _ _ _ => tt
         | Right _ _ _ => tt
         end b
@@ -43,7 +43,7 @@ Section htree.
                                    | Leaf _ => unit
                                    | Node l r => (path l -> B elm) -> (path r -> B elm) -> B elm
                                    end) with
-        | Finish => tt
+        | Stop => tt
         | Left _ _ p' => fun tget_l _ => tget_l p'
         | Right _ _ p' => fun _ tget_r => tget_r p'
         end (tget hl) (tget hr)
@@ -52,7 +52,7 @@ End htree.
 
 Implicit Arguments HLeaf [A B x].
 Implicit Arguments HNode [A B l r].
-Implicit Arguments Finish [A elm].
+Implicit Arguments Stop [A elm].
 Implicit Arguments Left [A elm l r].
 Implicit Arguments Right [A elm l r].
 
@@ -61,6 +61,47 @@ Example someTypes : tree Set :=
 Example someValues : htree (fun T : Set => T) someTypes :=
   HNode (HNode (HLeaf 42) (HLeaf tt)) (HLeaf true).
 
-Eval simpl in tget someValues (Right Finish).
-Eval simpl in tget someValues (Left (Right Finish)).
-Eval simpl in tget someValues (Left (Left Finish)).
+Eval simpl in tget someValues (Right Stop).
+Eval simpl in tget someValues (Left (Right Stop)).
+Eval simpl in tget someValues (Left (Left Stop)).
+
+Section htmap2.
+  Variable A : Type.
+  Variables B1 B2 C : A -> Type.
+  Variable f : forall x, B1 x -> B2 x -> C x.
+
+  Fixpoint htmap2 t (ht1 : htree B1 t) (ht2 : htree B2 t) : htree C t :=
+    match ht1 in htree _ t return htree _ t -> htree _ t with
+    | HLeaf x b1 => fun ht2 =>
+      match ht2
+            in htree _ t'
+            return
+            match t' with
+            | Leaf x' => B1 x' -> htree _ t'
+            | Node _ _ => B1 x -> unit
+            end
+      with
+      | HLeaf _ b2 => fun b1 => HLeaf (f b1 b2)
+      | HNode _ _ _ _ => fun _ => tt
+      end b1
+    | HNode l r hl1 hr1 => fun ht2 =>
+      match ht2
+            in htree _ t'
+            return
+            match t' with
+            | Leaf _ =>
+              (htree B2 l -> htree C l) ->
+              (htree B2 r -> htree C r) ->
+              unit
+            | Node l r =>
+              (htree B2 l -> htree C l) ->
+              (htree B2 r -> htree C r) ->
+              htree C (Node l r)
+            end
+      with
+      | HLeaf _ _ => fun _ _ => tt
+      | HNode _ _ hl2 hr2 =>
+        fun htmap2_l htmap2_r => HNode (htmap2_l hl2) (htmap2_r hr2)
+      end (htmap2 hl1) (htmap2 hr1)
+    end ht2.
+End htmap2.
